relax the typing constraint about the monad in the denote function

smallstep_monad.v
@@ -1,21 +1,27 @@
-(*
-  Denotation of the imperative language given in terms of the state/trace monad.
-  Prove that the small-step semantics is equivalent to the denotation.
-*)
-
 Require Import ssreflect ssrfun ssrbool Eqdep List.
 Import ListNotations.
 Require Import monad state_monad trace_monad smallstep.
 From mathcomp Require Import seq.
 
+(* contents:
+  Denotation of the imperative language given in terms of the state/trace monad.
+  Prove that the small-step semantics is equivalent to the denotation.
+  1. Section DenotationalSemantics
+  2. Section semantics_equivalence
+*)
+
 Set Bullet Behavior "Strict Subproofs".
+
+Set Implicit Arguments.
+Unset Strict Implicit.
+Unset Printing Implicit Defensive.
 
 Section DenotationalSemantics.
 
 Variables S T : Type.
-Variable M : stateTraceRunMonad S T.
+Variable M : stateTraceMonad S T.
 
-Fixpoint denote {A : Type} (p : program A) : M A :=
+Fixpoint denote A (p : program A) : M A :=
   match p with
   | p_ret _ v => Ret v
   | p_bind _ _ m f => do a <- denote m; denote (f a)
@@ -38,14 +44,14 @@ Fixpoint denote {A : Type} (p : program A) : M A :=
   end.
 
 Notation "'Repeat' n {{ p }}" := (
-  (fix loop (m : nat) : MonadStateTraceRun.m M unit :=
+  (fix loop (m : nat) : MonadStateTrace.m M unit :=
    match m with
    | 0 => Ret tt
    | Datatypes.S m' => denote p >> loop m'
    end) n) (at level 200).
 
 Notation "'While' fuel @ c {{ p }}" := (
-  (fix loop (m : nat) : MonadStateTraceRun.m M unit :=
+  (fix loop (m : nat) : MonadStateTrace.m M unit :=
    match m with
    | 0 => Ret tt
    | Datatypes.S m' =>
@@ -61,19 +67,28 @@ Fixpoint denote_continuation (k : continuation) : M (@continuation T S) :=
       denote_continuation (f a)
   end.
 
-Definition stateTrace_sub {A : Type} (m : M A) : Type :=
+Definition stateTrace_sub A (m : M A) : Type :=
   { p | denote p = m }.
 
 Definition continuation_sub (m : M continuation) : Type :=
   {k | denote_continuation k = m }.
+
+End DenotationalSemantics.
+
+Arguments denote {S} {T} M A.
+Arguments denote_continuation {S} {T} M.
+
+Section semantics_equivalence.
+
+Variables S T : Type.
+Variable M : stateTraceRunMonad S T.
 
 Lemma denote_prefix_preserved A (m : M A) :
   stateTrace_sub m -> forall s s' l1 l a,
   Run m (s, l1) = (a, (s', l)) ->
   exists l2, l = l1 ++ l2.
 Proof.
-intros [ p Hp ].
-subst m.
+case=> p <-{m}.
 induction p as [ A a | A B p IHp g IHg | A b p1 IHp1 p2 IHp2 |
   n p IHp | fuel c p IHp | | s0 | t ]; cbn;
  intros s s' l1 l a' Heq.
@@ -81,16 +96,13 @@ induction p as [ A a | A B p IHp g IHg | A b p1 IHp1 p2 IHp2 |
   rewrite cats0.
   by move: Heq; rewrite runret => -[].
 - rewrite runbind in Heq.
-  case_eq (Run (denote p) (s, l1)).
+  case_eq (Run (denote M _ p) (s, l1)).
   intros a (s0, l0) Hp.
   rewrite Hp in Heq.
-  apply IHp in Hp.
-  apply IHg in Heq.
-  destruct Hp as [l2 Hp].
-  destruct Heq as [l2' Heq].
+  move/IHp : Hp => [l2 Hp].
+  move/IHg : Heq => [l2' Heq].
   exists (l2 ++ l2').
-  rewrite catA.
-  congruence.
+  by rewrite Heq Hp catA.
 - destruct b; [ eapply IHp1 | eapply IHp2 ]; exact Heq.
 - revert s l1 Heq.
   induction n as [ | n' IH ]; intros s l1 Heq.
@@ -98,18 +110,14 @@ induction p as [ A a | A B p IHp g IHg | A b p1 IHp1 p2 IHp2 |
     rewrite cats0.
     by move: Heq; rewrite runret => -[].
   + rewrite runbind in Heq.
-    case_eq (Run (denote p) (s, l1)).
+    case_eq (Run (denote M _ p) (s, l1)).
     intros a (s0, l0) Hp.
-    specialize (IHp _ _ _ _ _ Hp).
-    destruct IHp as [l2 IHp ].
+    move: (IHp _ _ _ _ _ Hp) => [l2 ?].
     subst l0.
     rewrite Hp in Heq.
-    specialize (IH _ _ Heq).
-    destruct IH as [l3 IH].
+    move: (IH _ _ Heq) => [l3 ?].
     exists (l2 ++ l3).
-    subst l.
-    symmetry.
-    apply app_assoc.
+    by rewrite catA.
 - revert s l1 Heq.
   induction fuel as [ | fuel' IH ]; intros s l1 Heq.
   + exists [].
@@ -118,18 +126,14 @@ induction p as [ A a | A B p IHp g IHg | A b p1 IHp1 p2 IHp2 |
   + rewrite runbind runstget in Heq.
     destruct (c (s, l1).1).
     * rewrite runbind in Heq.
-      case_eq (Run (denote p) (s, l1)).
+      case_eq (Run (denote M _ p) (s, l1)).
       intros a (s0, l0) Hp.
-      specialize (IHp _ _ _ _ _ Hp).
-      destruct IHp as [l2 IHp ].
+      move: (IHp _ _ _ _ _ Hp) => [l2 ?].
       subst l0.
       rewrite Hp in Heq.
-      specialize (IH _ _ Heq).
-      destruct IH as [l3 IH].
+      move: (IH _ _ Heq) => [l3 ?].
       exists (l2 ++ l3).
-      subst l.
-      symmetry.
-      apply app_assoc.
+      by rewrite catA.
     * exists [].
       rewrite cats0.
       by move: Heq; rewrite runret => -[].
@@ -155,9 +159,9 @@ elim: p s l1 l2 => /= {A} [A a|A B p1 IH1 p2 IH2|A b p1 IH1 p2 IH2|
   n p IHp|fuel c p IHp||s'|t] s l1 l2.
 - by rewrite !runret.
 - rewrite [in LHS]runbind [in LHS]IH1.
-rewrite [in RHS]runbind.
-case: (Run (denote p1) (s, l2)) => a' [s' l'] /=.
-by rewrite IH2.
+  rewrite [in RHS]runbind.
+  case: (Run (denote M _ p1) (s, l2)) => a' [s' l'] /=.
+  by rewrite IH2.
 - by case: ifPn => _; [rewrite IH1|rewrite IH2].
 - revert s l2.
   induction n as [ | n' IH ]; intros s l2.
@@ -165,9 +169,9 @@ by rewrite IH2.
   + do 2 rewrite runbind.
     rewrite IHp.
     clear IHp.
-    case_eq (Run (denote p) (s, l2)).
+    case_eq (Run (denote M _ p) (s, l2)).
     intros a (s0, l0) Hp.
-    apply IH.
+    exact: IH.
 - revert s l2.
   induction fuel as [ | fuel' IH ]; intros s l2.
   + by rewrite !runret.
@@ -177,16 +181,16 @@ by rewrite IH2.
     * do 2 rewrite runbind.
       rewrite IHp.
       clear IHp.
-      case_eq (Run (denote p) (s, l2)).
+      case_eq (Run (denote M _ p) (s, l2)).
       intros a (s0, l0) Hp.
-      apply IH.
+      exact: IH.
     * by rewrite !runret.
 - by rewrite !runstget.
 - by rewrite !runstput.
 - by rewrite !runstmark rcons_cat.
 Qed.
 
-Lemma denote_continuation_prefix_independent m :
+Lemma denote_continuation_prefix_independent (m : M _) :
   continuation_sub m -> forall s l1 l2,
   Run m (s, l1 ++ l2) =
   let res := Run m (s, l2) in
@@ -198,13 +202,13 @@ elim: k => // [A a s l1 l2|A p k IH s l1 l2].
 by rewrite !runret.
 rewrite /= !runbind.
 rewrite denote_prefix_independent /=; [ | now exists p ].
-destruct (Run (denote p) (s, l2)) as [ a (s', l) ].
+destruct (Run (denote M _ p) (s, l2)) as [ a (s', l) ].
 by rewrite IH.
 Qed.
 
 Lemma step_None_correct s s' k k' l :
   step (s, k) None (s', k') ->
-  Run (denote_continuation k) (s, l) = Run (denote_continuation k') (s', l).
+  Run (denote_continuation M k) (s, l) = Run (denote_continuation M k') (s', l).
 Proof.
 intro Hstep.
 remember (s, k) as sk eqn: Heq.
@@ -254,8 +258,8 @@ Qed.
 
 Lemma step_Some_correct s s' k k' t l :
   step (s, k) (Some t) (s', k') ->
-  Run (denote_continuation k) (s, l) =
-  Run (denote_continuation k') (s', rcons l t).
+  Run (denote_continuation M k) (s, l) =
+  Run (denote_continuation M k') (s', rcons l t).
 Proof.
 intro Hstep.
 remember (s, k) as sk eqn: Heq.
@@ -274,7 +278,7 @@ Qed.
 
 Lemma step_star_correct_gen s s' k k' l l' :
   step_star (s, k) l' (s', k') ->
-  Run (denote_continuation k) (s, l) = Run (denote_continuation k') (s', l++l').
+  Run (denote_continuation M k) (s, l) = Run (denote_continuation M k') (s', l++l').
 Proof.
 intro Hstep_star.
 remember (s, k) as sk eqn: Heq.
@@ -286,15 +290,12 @@ induction Hstep_star as
   (s, k) (s', k') (s'', k'') t l' Hstep Hstep_star IH ];
  intros s1 s2 k1 k2 l1 Heq1 Heq2.
 - rewrite cats0.
-  rewrite Heq1 in Heq2.
-  injection Heq2; intros; subst; reflexivity.
-- injection Heq1; clear Heq1; intros; subst s1 k1.
-  injection Heq2; clear Heq2; intros; subst s2 k2.
+  by move: Heq2; rewrite Heq1 => -[<- <-].
+- move: Heq1 Heq2 => [<- <-] [<- <-].
   apply step_None_correct with (l := l1) in Hstep.
   rewrite Hstep.
   apply IH; reflexivity.
-- injection Heq1; clear Heq1; intros; subst s1 k1.
-  injection Heq2; clear Heq2; intros; subst s2 k2.
+- move: Heq1 Heq2 => [<- <-] [<- <-].
   apply step_Some_correct with (l := []) in Hstep.
   rewrite <- cats0 at 1.
   rewrite denote_continuation_prefix_independent; [ | now exists k ].
@@ -308,22 +309,21 @@ Qed.
 Proposition step_star_correct
   (s s' : S) (A : Type) (a : A) (p : program A) (l : list T) :
   step_star (s, p `; stop A) l (s', stop A a) ->
-  Run (denote p) (s, []) = (a, (s', l)).
+  Run (denote M _ p) (s, []) = (a, (s', l)).
 Proof.
 intro Hss.
 apply step_star_correct_gen with (l := []) in Hss.
 move: Hss.
 rewrite /= runret runbind.
-destruct (Run (denote p) (s, [])) as [a'' [s'' l'']].
-rewrite runret => Hss.
-injection Hss; clear Hss; intros Heq1 Heq2 Heq3.
+destruct (Run (denote M _ p) (s, [])) as [a'' [s'' l'']].
+rewrite runret => -[Heq3 <- <-].
 apply inj_pair2 in Heq3.
-congruence.
+by rewrite Heq3.
 Qed.
 
 Lemma step_star_complete_gen
   (s s' : S) (A : Type) (a : A) (p : program A) (l1 l2 : list T) f :
-  Run (denote p) (s, l1) = (a, (s', l1 ++ l2)) ->
+  Run (denote M _ p) (s, l1) = (a, (s', l1 ++ l2)) ->
   step_star (s, p `; f) l2 (s', f a).
 Proof.
 revert s s' a l1 l2 f.
@@ -339,15 +339,13 @@ induction p as [ A a | A B p IHp g IHg | A b p1 IHp1 p2 IHp2 |
   + apply s_bind.
   + move: Heq.
     rewrite runbind.
-    case_eq (Run (denote p) (s, l1)).
+    case_eq (Run (denote M _ p) (s, l1)).
     intros a (s0, l0) Hp Heq.
-    specialize (denote_prefix_preserved _ _ ltac:(now eexists) _ _ _ _ _ Hp).
-    intros [l3 Hl3].
+    move: (denote_prefix_preserved ltac:(now eexists) Hp) => [l3 Hl3].
     rewrite Hl3 in Hp.
     apply IHp with (f := (fun a => g a `; f)) in Hp.
     clear IHp.
-    specialize (denote_prefix_preserved _ _ ltac:(now eexists) _ _ _ _ _ Heq).
-    intros [l4 Hl4].
+    move: (denote_prefix_preserved ltac:(now eexists) Heq) => [l4 Hl4].
     rewrite Hl4 in Heq.
     apply IHg with (f := f) in Heq.
     clear IHg.
@@ -355,7 +353,7 @@ induction p as [ A a | A B p IHp g IHg | A b p1 IHp1 p2 IHp2 |
     replace l2 with (l3 ++ l4) by
      (induction l1; cbn in Hl4; [ congruence | injection Hl4; tauto ]).
     eapply step_star_transitive.
-    * apply Hp.
+    * exact Hp.
     * exact Heq.
 - destruct b; [
     eapply ss_step_None; [
@@ -373,32 +371,20 @@ induction p as [ A a | A B p IHp g IHg | A b p1 IHp1 p2 IHp2 |
      (revert l2 H; induction l1; [ tauto | intros ? [=]; firstorder ]).
     eapply ss_step_None; [ apply s_repeat_O | apply ss_refl ].
   + rewrite runbind in Heq.
-    case_eq (Run (denote p) (s, l1)).
+    case_eq (Run (denote M _ p) (s, l1)).
     intros a (s0, l0) Hp.
     rewrite Hp in Heq.
-    specialize (denote_prefix_preserved _ _ ltac:(now eexists) _ _ _ _ _ Hp).
-    intros [l3 Hl3].
-    rewrite Hl3 in Hp, Heq.
-    clear l0 Hl3.
+    move: (denote_prefix_preserved ltac:(now eexists) Hp) => [l3 Hl3].
+    rewrite Hl3 {l0 Hl3} in Hp, Heq.
     specialize (IHp _ _ _ _ _ (fun _ => p_repeat n' p `; f) Hp).
     assert (Heq':
-     Run (denote (p_repeat n' p)) (s0, l1 ++ l3) = (a', (s', l1 ++ l2)))
+     Run (denote M _ (p_repeat n' p)) (s0, l1 ++ l3) = (a', (s', l1 ++ l2)))
      by apply Heq.
-    specialize (denote_prefix_preserved _ _ ltac:(now eexists) _ _ _ _ _ Heq').
-    intros [l4 Hl4].
+    move: (denote_prefix_preserved ltac:(now eexists) Heq') => [l4 Hl4].
     rewrite Hl4 in Heq.
     eapply ss_step_None; [ apply s_repeat_S | ].
-    assert (Hl2: l2 = l3 ++ l4).
-    {
-      revert Hl4.
-      clear.
-      induction l1 as [ | a1 l1 IH ]; [ trivial | ].
-      cbn.
-      intro H.
-      apply IH.
-      injection H; trivial.
-    }
-    rewrite Hl2.
+    have -> : l2 = l3 ++ l4.
+      by move/(congr1 (drop (size l1))) : Hl4; rewrite -catA ?drop_size_cat.
     eapply step_star_transitive; [ eexact IHp | eapply IHn; eexact Heq ].
 - revert s l1 l2 Heq.
   induction fuel as [ | fuel' IHn ]; intros s l1 l2 Heq.
@@ -411,58 +397,42 @@ induction p as [ A a | A B p IHp g IHg | A b p1 IHp1 p2 IHp2 |
     cbn in Heq.
     case_eq (c s); [ intro Htrue | intro Hfalse ].
     * rewrite Htrue runbind in Heq.
-      case_eq (Run (denote p) (s, l1)).
+      case_eq (Run (denote M _ p) (s, l1)).
       intros a (s0, l0) Hp.
       rewrite Hp in Heq.
-      specialize (denote_prefix_preserved _ _ ltac:(now eexists) _ _ _ _ _ Hp).
-      intros [l3 Hl3].
-      rewrite Hl3 in Hp, Heq.
-      clear l0 Hl3.
+      move: (denote_prefix_preserved ltac:(now eexists) Hp) => [l3 Hl3].
+      rewrite Hl3 {l0 Hl3} in Hp, Heq.
       specialize (IHp _ _ _ _ _ (fun _ => p_while fuel' c p `; f) Hp).
       assert (Heq':
-       Run (denote (p_while fuel' c p)) (s0, l1 ++ l3) = (a', (s', l1 ++ l2)))
+       Run (denote M _ (p_while fuel' c p)) (s0, l1 ++ l3) = (a', (s', l1 ++ l2)))
        by apply Heq.
-      specialize (denote_prefix_preserved _ _ ltac:(now eexists) _ _ _ _ _ Heq').
-      intros [l4 Hl4].
+      move: (denote_prefix_preserved ltac:(now eexists) Heq') => [l4 Hl4].
       rewrite Hl4 in Heq.
       eapply ss_step_None; [ apply s_while_true; exact Htrue | ].
-      assert (Hl2: l2 = l3 ++ l4).
-      {
-        revert Hl4.
-        clear.
-        induction l1 as [ | a1 l1 IH ]; [ trivial | ].
-        cbn.
-        intro H.
-        apply IH.
-        injection H; trivial.
-      }
-      rewrite Hl2.
+      have -> : l2 = l3 ++ l4.
+        by move/(congr1 (drop (size l1))) : Hl4; rewrite -catA ?drop_size_cat.
       eapply step_star_transitive; [ eexact IHp | eapply IHn; eexact Heq ].
-    * rewrite Hfalse runret in Heq.
-      injection Heq; clear Heq; intros; subst a' s'.
-      replace l2 with (@nil T) by
-       (revert l2 H; induction l1; [ tauto | intros ? [=]; firstorder ]).
+    * move: Heq; rewrite Hfalse runret.
+      move=> [<- <-] /(congr1 (drop (size l1))).
+      rewrite drop_size_cat // drop_size => <-.
       eapply ss_step_None; [ apply s_while_false; exact Hfalse | apply ss_refl ].
-- rewrite runstget in Heq.
-  injection Heq; clear Heq; intros; subst a' s'.
-  replace l2 with (@nil T) by
-   (revert l2 H; induction l1; [ tauto | intros ? [=]; firstorder ]).
+- move: Heq; rewrite runstget.
+  move=> [<- <-] /(congr1 (drop (size l1))).
+  rewrite drop_size_cat // drop_size => <-.
   eapply ss_step_None; [ apply s_get | apply ss_refl ].
-- rewrite runstput in Heq.
-  injection Heq; clear Heq; intros; subst a' s'.
-  replace l2 with (@nil T) by
-   (revert l2 H; induction l1; [ tauto | intros ? [=]; firstorder ]).
+- move: Heq; rewrite runstput.
+  move=> [<- <-] /(congr1 (drop (size l1))).
+  rewrite drop_size_cat // drop_size => <-.
   eapply ss_step_None; [ apply s_put | apply ss_refl ].
-- rewrite runstmark in Heq.
-  injection Heq; clear Heq; intros; subst a' s'.
-  replace l2 with [t] by
-   (revert l2 H; induction l1; [ tauto | intros ? [=]; firstorder ]).
+- move: Heq; rewrite runstmark.
+  move=> [<- <-] /(congr1 (drop (size l1))).
+  rewrite drop_size_cat // drop_rcons // drop_size => <-.
   eapply ss_step_Some; [ apply s_mark | apply ss_refl ].
 Qed.
 
 Proposition step_star_complete
   (s s' : S) (A : Type) (a : A) (p : program A) (l : list T) :
-  Run (denote p) (s, []) = (a, (s', l)) ->
+  Run (denote M _ p) (s, []) = (a, (s', l)) ->
   step_star (s, p `; stop A) l (s', stop A a).
 Proof.
 intro Hp.
@@ -470,6 +440,4 @@ apply step_star_complete_gen with (l1 := []).
 exact Hp.
 Qed.
 
-End DenotationalSemantics.
-
-Arguments denote [S] [T] _ _.
+End semantics_equivalence.
